src/lowparse/LowParse.SteelST.VCList.fst
@@ -1,0 +1,305 @@
+module LowParse.SteelST.VCList
+include LowParse.SteelST.List.Base
+include LowParse.SteelST.Parse // to shadow the vl vs. v operators from List
+include LowParse.Spec.VCList
+open Steel.ST.GenElim
+
+module AP = LowParse.SteelST.ArrayPtr
+
+let aparse_nlist_aparse_list
+  (#opened: _)
+  (#k: parser_kind)
+  (#t: Type)
+  (p: parser k t)
+  (n: nat)
+  (#va: v (parse_nlist_kind n k) (nlist n t))
+  (a: byte_array)
+: STGhost (v parse_list_kind (list t)) opened
+    (aparse (parse_nlist n p) a va)
+    (fun va' -> aparse (parse_list p) a va')
+    (k.parser_kind_low > 0)
+    (fun va' ->
+      array_of va' == array_of va /\
+      va'.contents == (va.contents <: list t)
+    )
+= let b = elim_aparse _ a in
+  parse_nlist_parse_list_full p n (AP.contents_of b);
+  intro_aparse _ a
+
+let aparse_list_aparse_nlist
+  (#opened: _)
+  (#k: parser_kind)
+  (#t: Type)
+  (p: parser k t)
+  (n: nat)
+  (#va: v parse_list_kind (list t))
+  (a: byte_array)
+: STGhost (v (parse_nlist_kind n k) (nlist n t)) opened
+    (aparse (parse_list p) a va)
+    (fun va' -> aparse (parse_nlist n p) a va')
+    (n == List.Tot.length va.contents)
+    (fun va' ->
+      array_of' va' == array_of' va /\
+      (va'.contents <: list t) == va.contents
+    )
+= let b = elim_aparse _ a in
+  parse_list_parse_nlist p (AP.contents_of b);
+  intro_aparse _ a
+
+let intro_nlist_nil
+  (#opened: _)
+  (#k: parser_kind)
+  (#t: Type)
+  (n: nat)
+  (p: parser k t)
+  (#va: _)
+  (a: byte_array)
+: STGhost (v (parse_nlist_kind n k) (nlist n t)) opened
+    (AP.arrayptr a va)
+    (fun va' -> aparse (parse_nlist n p) a va')
+    (AP.length (AP.array_of va) == 0 /\
+      n == 0
+    )
+    (fun va' ->
+      array_of va' == AP.array_of va /\
+      va'.contents == []
+    )
+= parse_nlist_zero p (AP.contents_of va);
+  intro_aparse (parse_nlist n p) a
+
+let elim_nlist_nil
+  (#opened: _)
+  (#k: parser_kind)
+  (#t: Type)
+  (n: nat)
+  (p: parser k t)
+  (#va: v (parse_nlist_kind n k) (nlist n t))
+  (a: byte_array)
+: STGhost (AP.v byte) opened
+    (aparse (parse_nlist n p) a va)
+    (fun va' -> AP.arrayptr a va')
+    (n == 0 \/ Nil? va.contents)
+    (fun va' ->
+      n == 0 /\
+      Nil? va.contents /\
+      array_of va == AP.array_of va' /\
+      AP.length (AP.array_of va') == 0
+    )
+= let va' = elim_aparse (parse_nlist n p) a in
+  parse_nlist_zero p (AP.contents_of va');
+  noop ();
+  va'
+
+let intro_nlist_cons
+  (#opened: _)
+  (#k: parser_kind)
+  (#t: Type)
+  (n': nat)
+  (p: parser k t)
+  (n: nat)
+  (#va1: v _ _)
+  (#va2: v _ _)
+  (a1 a2: byte_array)
+: STGhost (v (parse_nlist_kind n' k) (nlist n' t)) opened
+    (aparse p a1 va1 `star` aparse (parse_nlist n p) a2 va2)
+    (fun va -> aparse (parse_nlist n' p) a1 va)
+    (k.parser_kind_subkind == Some ParserStrong /\
+      k.parser_kind_low > 0 /\
+      AP.adjacent (array_of va1) (array_of va2) /\
+      n' == n + 1
+    )
+    (fun va ->
+      n' == n + 1 /\
+      AP.merge_into (array_of' va1) (array_of' va2) (array_of' va) /\
+      va.contents == va1.contents :: va2.contents
+    )
+= let _ = aparse_nlist_aparse_list p n a2 in
+  let _ = intro_cons p a1 a2 in
+  aparse_list_aparse_nlist p n' a1
+
+let list_length_cons
+  (#t: Type)
+  (a: t)
+  (q: list t)
+: Lemma
+  (List.Tot.length (a :: q) == 1 + List.Tot.length q)
+= ()
+
+let list_length_cons_n
+  (#t: Type)
+  (a: t)
+  (q: list t)
+  (n: nat)
+  (n_pred: nat)
+: Lemma
+  (requires (List.Tot.length (a :: q) == n /\
+    n == n_pred + 1))
+  (ensures (List.Tot.length q == n_pred))
+= ()
+
+let elim_nlist_cons_post
+  (k: parser_kind)
+  (t: Type0)
+  (n n_pred: nat)
+  (va1: v k t) (va2: v (parse_nlist_kind n_pred k) (nlist n_pred t))
+  (va: v (parse_nlist_kind n k) (nlist n t))
+: GTot prop
+=
+      n == n_pred + 1 /\
+      AP.merge_into (array_of va1) (array_of va2) (array_of va) /\
+      va.contents == va1.contents :: va2.contents /\
+      AP.length (array_of va1) > 0
+
+#push-options "--z3rlimit 32 --z3cliopt smt.arith.nl=false"
+
+#restart-solver
+let elim_nlist_cons
+  (#opened: _)
+  (#k: parser_kind)
+  (#t: Type0)
+  (p: parser k t)
+  (n: nat)
+  (n_pred: nat)
+  (#va: v _ _)
+  (a: byte_array)
+: STGhost (Ghost.erased byte_array) opened
+    (aparse (parse_nlist n p) a va)
+    (fun a2 -> exists_ (fun (va1: v _ _) -> exists_ (fun (va2: v _ _) ->
+      aparse p a va1 `star`
+      aparse (parse_nlist n_pred p) a2 va2 `star` pure (
+      elim_nlist_cons_post k t n n_pred va1 va2 va
+    ))))
+    (Cons? va.contents /\
+      n == n_pred + 1 /\
+      k.parser_kind_low > 0 /\
+      k.parser_kind_subkind == Some ParserStrong)
+    (fun _ -> True)
+= let _ = aparse_nlist_aparse_list p n a in
+  let a2 = ghost_elim_cons p a in
+  let _ = gen_elim () in
+  let va1 = vpattern_replace (aparse p a) in
+  let va2 = vpattern_replace (aparse (parse_list p) a2) in
+  list_length_cons_n va1.contents va2.contents n n_pred; 
+  noop ();
+  let _ = aparse_list_aparse_nlist p n_pred a2 in
+  noop ();
+  a2
+
+#pop-options
+
+let rec intro_nlist_sum
+  (#opened: _)
+  (#k: parser_kind)
+  (#t: Type)
+  (n: nat)
+  (p: parser k t)
+  (n1: nat)
+  (#va1: v (parse_nlist_kind n1 k) (nlist n1 t))
+  (a1: byte_array)
+  (n2: nat)
+  (#va2: v (parse_nlist_kind n2 k) (nlist n2 t))
+  (a2: byte_array)
+: STGhost (v (parse_nlist_kind n k) (nlist n t)) opened
+    (aparse (parse_nlist n1 p) a1 va1 `star` aparse (parse_nlist n2 p) a2 va2)
+    (fun va' -> aparse (parse_nlist n p) a1 va')
+    (AP.adjacent (array_of' va1) (array_of' va2) /\
+      k.parser_kind_low > 0 /\
+      n == n1 + n2 /\
+      k.parser_kind_subkind == Some ParserStrong
+    )
+    (fun va' ->
+      AP.merge_into (array_of' va1) (array_of' va2) (array_of' va') /\
+      va'.contents == va1.contents `List.Tot.append` va2.contents
+    )
+    (decreases n1)
+= if n1 = 0
+  then begin
+    let va1' = elim_nlist_nil n1 p a1 in
+    let va2' = elim_aparse (parse_nlist n2 p) a2 in
+    let va' = AP.join a1 a2 in
+    assert (AP.contents_of va' `Seq.equal` AP.contents_of va2');
+    noop ();
+    intro_aparse (parse_nlist n p) a1
+  end else begin
+    noop ();
+    let n1' : nat = n1 - 1 in
+    let n' : nat = n - 1 in
+    let a1' = elim_nlist_cons p n1 n1' a1 in
+    let _ = gen_elim () in
+    let _ = intro_nlist_sum n' p n1' a1' n2 a2 in
+    let res = intro_nlist_cons n p n' a1 a1' in
+    res
+  end
+
+let elim_nlist_sum_post
+  (t: Type)
+  (k: parser_kind)
+  (n n1 n2: nat)
+  (va1: v (parse_nlist_kind n1 k) (nlist n1 t))
+  (va2: v (parse_nlist_kind n2 k) (nlist n2 t))
+  (va: v (parse_nlist_kind n k) (nlist n t))
+: GTot prop
+=
+        n == n1 + n2 /\
+        AP.merge_into (array_of' va1) (array_of' va2) (array_of' va) /\
+        va.contents == va1.contents `List.Tot.append` va2.contents
+
+#push-options "--z3rlimit 16"
+
+#restart-solver
+let rec elim_nlist_sum
+  (#opened: _)
+  (#k: parser_kind)
+  (#t: Type)
+  (n: nat)
+  (p: parser k t)
+  (#va: v (parse_nlist_kind n k) (nlist n t))
+  (a: byte_array)
+  (n1 n2: nat)
+: STGhost (Ghost.erased byte_array) opened
+    (aparse (parse_nlist n p) a va)
+    (fun ar -> exists_ (fun va1 -> exists_ (fun va2 ->
+      aparse (parse_nlist n1 p) a va1 `star` aparse (parse_nlist n2 p) ar va2 `star`
+      pure (elim_nlist_sum_post t k n n1 n2 va1 va2 va)
+    )))
+    (k.parser_kind_low > 0 /\
+      n == n1 + n2 /\
+      k.parser_kind_subkind == Some ParserStrong
+    )
+    (fun _ -> True)
+    (decreases n1)
+=
+  if n1 = 0
+  then begin
+    let va = elim_aparse (parse_nlist n p) a in
+    let ar = AP.gsplit a 0sz in
+    let _ = gen_elim () in
+    let vr = vpattern_replace (AP.arrayptr ar) in
+    assert (AP.contents_of' vr `Seq.equal` AP.contents_of' va);
+    let _ = intro_nlist_nil n1 p a in
+    let _ = intro_aparse (parse_nlist n2 p) ar in
+    noop ();
+    ar
+  end else begin
+    let n1' : nat = n1 - 1 in
+    let n' : nat = n - 1 in
+    let a' = elim_nlist_cons p n n' a in
+    let _ = gen_elim () in
+    let ar = elim_nlist_sum n' p a' n1' n2 in
+    let _ = gen_elim () in
+    let _ = intro_nlist_cons n1 p n1' a a' in
+    noop ();
+    ar
+  end
+
+#pop-options
+
+let aparse_nlist_count_le_size
+  (k: parser_kind)
+  (t: Type)
+  (n: nat)
+  (va: v (parse_nlist_kind n k) (nlist n t))
+: Lemma
+  (requires (k.parser_kind_low > 0))
+  (ensures (n <= AP.length (array_of' va)))
+= ()
